A proof of spec equivalence between repeat_blocks and update_multi style specifications

code/streaming/Hacl.Streaming.Lemmas.fst
@@ -4,18 +4,30 @@ module Hacl.Streaming.Lemmas
 /// for specifications in the streaming functor, and the lib-based repeat
 /// imperative combinators.
 
-#set-options "--max_fuel 0 --max_ifuel 0 --z3rlimit 100"
-let rec update_multi_is_repeat_blocks #a block_length update update_last acc input =
+/// This is the reason why repeat_l is hoisted
+let repeat_l_input #a (block_length:pos { block_length < pow2 32 })
+  (update_last: (a -> s:S.seq uint8 { S.length s < block_length } -> a))
+  (input1 input2:S.seq uint8)
+  (l: Lib.IntTypes.size_nat { l == S.length input1 % block_length })
+  (s: Lib.Sequence.lseq uint8 l)
+  (acc: a): Lemma
+    (requires S.length input1 % block_length == S.length input2 % block_length)
+    (ensures repeat_l block_length update_last input1 l s acc ==
+      repeat_l block_length update_last input2 l s acc)
+  [ SMTPat (repeat_l block_length update_last input1 l s acc);
+    SMTPat (repeat_l block_length update_last input2 l s acc) ]
+=
+  ()
+
+#set-options "--z3rlimit 300"
+let rec update_multi_is_repeat_blocks #a block_length update update_last acc input input' =
   // Spec.UpdateMulti side
   let n_blocks = S.length input / block_length in
   let blocks, rest = S.split input (n_blocks * block_length) in
 
   // Lib.Sequence side
-  let repeat_f = fun (input: S.seq uint8 { S.length input = block_length }) (acc: a) -> update acc input in
-  let repeat_l = fun (l: Lib.IntTypes.size_nat { l == S.length input % block_length })
-    (s: Lib.Sequence.lseq uint8 l) (acc: a) ->
-    update_last acc s
-  in
+  let repeat_f = repeat_f block_length update in
+  let repeat_l = repeat_l block_length update_last input' in
   let repeat_acc =
     Lib.LoopCombinators.repeati n_blocks (Lib.Sequence.repeat_blocks_f block_length input repeat_f n_blocks) acc
   in
@@ -42,8 +54,11 @@ let rec update_multi_is_repeat_blocks #a block_length update update_last acc inp
     assert (repeat_final_acc == update_full block_length update update_last acc input)
   end else begin
     let head, tail = Spec.UpdateMulti.split_block block_length blocks 1 in
+    assert (S.length head % block_length = 0);
     S.lemma_eq_intro (head `S.append` tail `S.append` rest) input;
     S.lemma_eq_intro (head `S.append` (tail `S.append` rest)) input;
+    S.lemma_eq_intro (S.slice input 0 block_length) head;
+    S.lemma_eq_intro (S.slice input block_length (S.length input)) (tail `S.append` rest);
     S.lemma_len_append head (tail `S.append` rest);
     S.lemma_len_append tail rest;
     calc (==) {
@@ -57,6 +72,7 @@ let rec update_multi_is_repeat_blocks #a block_length update update_last acc inp
     };
     S.lemma_eq_intro (fst (S.split (tail `S.append` rest) ((n_blocks - 1) * block_length))) tail;
     S.lemma_eq_intro (snd (S.split (tail `S.append` rest) ((n_blocks - 1) * block_length))) rest;
+    assert (S.length (tail `S.append` rest) % block_length == S.length input % block_length);
 
     norm_spec [zeta; iota; primops; delta_only [`%mk_update_multi]]
       (mk_update_multi block_length update acc (head `S.append` tail));
@@ -66,13 +82,22 @@ let rec update_multi_is_repeat_blocks #a block_length update update_last acc inp
       update_last (mk_update_multi block_length update (update acc head) tail) rest;
     (==) { }
       update_full block_length update update_last (update acc head) (tail `S.append` rest);
-    };
+    (==) { update_multi_is_repeat_blocks #a block_length update update_last (update acc head) (tail `S.append` rest) input' }
+      Lib.Sequence.repeat_blocks #uint8 block_length (tail `S.append` rest) repeat_f repeat_l (update acc head);
+    (==) { }
+      Lib.Sequence.repeat_blocks #uint8 block_length (tail `S.append` rest) repeat_f repeat_l (repeat_f head acc);
+    (==) {
+      Lib.LoopCombinators.eq_repeati0 1 (Lib.Sequence.repeat_blocks_f block_length head repeat_f 1) acc;
+      Lib.LoopCombinators.unfold_repeati 1 (Lib.Sequence.repeat_blocks_f block_length head repeat_f 1) acc 0
+    }
+      Lib.Sequence.repeat_blocks #uint8 block_length (tail `S.append` rest) repeat_f repeat_l
+        (Lib.LoopCombinators.repeati 1 (Lib.Sequence.repeat_blocks_f block_length head repeat_f 1) acc);
 
-    update_multi_is_repeat_blocks #a block_length update update_last (update acc head) (tail `S.append` rest);
-    assert (update_full block_length update update_last (update acc head) (tail `S.append` rest) ==
-      Lib.Sequence.repeat_blocks #uint8 block_length (tail `S.append` rest) repeat_f repeat_l (update acc head));
+    (==) { Lib.Sequence.lemma_repeat_blocks_multi block_length head repeat_f acc }
+      Lib.Sequence.repeat_blocks #uint8 block_length (tail `S.append` rest) repeat_f repeat_l
+        (Lib.Sequence.repeat_blocks_multi block_length head repeat_f acc);
 
-    Lib.LoopCombinators.unfold_repeati n_blocks
-      (Lib.Sequence.repeat_blocks_f block_length input repeat_f n_blocks) acc (n_blocks - 1);
-    admit ()
+    (==) { Lib.Sequence.Lemmas.repeat_blocks_split block_length block_length input repeat_f repeat_l acc }
+      Lib.Sequence.repeat_blocks #uint8 block_length input repeat_f repeat_l acc;
+    }
   end
